examples/proofs/intptr/generated_spec.v
@@ -76,6 +76,6 @@ Section spec.
 
   (* Specifications for function [int_to_ptr]. *)
   Definition type_of_int_to_ptr :=
-    fn(∀ p : loc; (p @ (intptr (uintptr_t))); True)
-      → ∃ () : (), (p @ (&own (place (p)))); True.
+    fn(∀ p : loc; (p @ (intptr (uintptr_t))); (alloc_alive_loc p) ∗ (loc_in_bounds p 0))
+      → ∃ () : (), (p @ (&own (place (p)))); (alloc_alive_loc p).
 End spec.
