theories/lang/lifting.v
@@ -373,10 +373,19 @@ Qed.
 Lemma wp_copy_alloc_id Φ l1 l2 v1 v2 E:
   val_to_loc v1 = Some l1 →
   val_to_loc v2 = Some l2 →
-  ▷ Φ (val_of_loc (l2.1, l1.2)) -∗ WP CopyAllocId PtrOp (Val v1) (Val v2) @ E {{ Φ }}.
+  loc_in_bounds (l2.1, l1.2) 0 -∗
+  alloc_alive_loc l2 ∧ ▷ Φ (val_of_loc (l2.1, l1.2)) -∗
+  WP CopyAllocId PtrOp (Val v1) (Val v2) @ E {{ Φ }}.
 Proof.
-  iIntros (Hl1 Hl2) "HΦ". iApply wp_lift_expr_step => //.
-  iIntros (σ1) "Hctx !>". iSplit; first by eauto 8 using CopyAllocIdPS.
+  iIntros (Hl1 Hl2) "Hl HΦ". iApply wp_lift_expr_step => //.
+  iIntros (σ1) "Hctx !>".
+  iAssert ⌜valid_ptr (l2.1, l1.2) σ1.(st_heap)⌝%I as %?. {
+    iSplit; [ |iApply (loc_in_bounds_to_heap_loc_in_bounds with "Hl Hctx")].
+    iApply (alloc_alive_loc_to_block_alive with "[HΦ] Hctx").
+    iDestruct "HΦ" as "[Halive _]". by iApply alloc_alive_loc_mono; [|done].
+  }
+  iDestruct "HΦ" as "[_ HΦ]".
+  iSplit; first by eauto 8 using CopyAllocIdPS.
   iIntros "!>" (???? Hstep ?) "!>". inv_expr_step. iSplit => //. iFrame.
   by iApply wp_value.
 Qed.
@@ -384,10 +393,19 @@ Qed.
 Lemma wp_copy_alloc_id_int Φ it l1 l2 v1 v2 E:
   val_to_loc v1 = Some l1 →
   val_to_loc_weak v2 it = Some l2 →
-  ▷ Φ (val_of_loc (l2.1, l1.2)) -∗ WP CopyAllocId (IntOp it) (Val v1) (Val v2) @ E {{ Φ }}.
+  loc_in_bounds (l2.1, l1.2) 0 -∗
+  alloc_alive_loc l2 ∧ ▷ Φ (val_of_loc (l2.1, l1.2)) -∗
+  WP CopyAllocId (IntOp it) (Val v1) (Val v2) @ E {{ Φ }}.
 Proof.
-  iIntros (Hl1 Hl2) "HΦ". iApply wp_lift_expr_step => //.
-  iIntros (σ1) "Hctx !>". iSplit; first by eauto 8 using CopyAllocIdIS.
+  iIntros (Hl1 Hl2) "Hl HΦ". iApply wp_lift_expr_step => //.
+  iIntros (σ1) "Hctx !>".
+  iAssert ⌜valid_ptr (l2.1, l1.2) σ1.(st_heap)⌝%I as %?. {
+    iSplit; [ |iApply (loc_in_bounds_to_heap_loc_in_bounds with "Hl Hctx")].
+    iApply (alloc_alive_loc_to_block_alive with "[HΦ] Hctx").
+    iDestruct "HΦ" as "[Halive _]". by iApply alloc_alive_loc_mono; [|done].
+  }
+  iDestruct "HΦ" as "[_ HΦ]".
+  iSplit; first by eauto 8 using CopyAllocIdIS.
   iIntros "!>" (???? Hstep ?) "!>". inv_expr_step. iSplit => //. iFrame.
   by iApply wp_value.
 Qed.
@@ -469,10 +487,8 @@ Proof.
   }
   rewrite Hv /=. move: Hv => /val_to_of_Z Hv.
   iApply wp_ptr_offset; [done| by apply: val_to_Z_to_int_repr_Z | | ].
-  { have ? := offset_of_idx_le_size sl i.
-    have -> : (ly_size sl = offset_of_idx (sl_members sl) i + (ly_size sl - offset_of_idx (sl_members sl) i))%nat by lia.
-    rewrite -loc_in_bounds_split offset_loc_sz1 //.
-    iDestruct "Hl" as "[_ Hl]". iApply (loc_in_bounds_shorten with "Hl"). lia. }
+  { have ? := offset_of_idx_le_size sl i. rewrite offset_loc_sz1 //.
+    iApply (loc_in_bounds_offset with "Hl"); simpl; [done| destruct l => /=; lia  | destruct l => /=; lia ]. }
   by rewrite offset_loc_sz1.
 Qed.
 Lemma wp_get_member_union Φ vl l ul n E:
