theories/typing/intptr.v
@@ -129,6 +129,8 @@ Section programs.
   Lemma type_copy_aid_intptr v1 P1 v2 p2 it T:
     (∃ p1,
       subsume P1 (v1 ◁ᵥ p1 @ frac_ptr Own (place p1)) (
+        (loc_in_bounds (p2.1, p1.2) 0 ∗ True) ∧
+        (alloc_alive_loc p2 ∗ True) ∧
         T (val_of_loc (p2.1, p1.2)) (t2mt (value void* (val_of_loc (p2.1, p1.2))))
       )
     ) -∗
@@ -137,8 +139,10 @@ Section programs.
     iIntros "HT Hp1 Hp2" (Φ) "HΦ". iDestruct "HT" as (p1) "HT".
     iDestruct ("HT" with "Hp1") as "[Hp1 HT]". iDestruct "Hp1" as (->) "Hp1".
     iDestruct "Hp2" as %Hp2.
+    rewrite !right_id. iDestruct "HT" as "[#Hlib HT]".
     iApply wp_copy_alloc_id_int => //; first by rewrite val_to_of_loc.
-    by iApply ("HΦ" with "[] HT").
+    iSplit; [by iDestruct "HT" as "[$ _]" |].
+    iDestruct "HT" as "[_ HT]". by iApply ("HΦ" with "[] HT").
   Qed.
   Global Instance type_copy_aid_intptr_inst v1 P1 v2 p2 it:
     TypedCopyAllocId v1 P1 v2 (v2 ◁ᵥ p2 @ intptr it)%I (IntOp it) :=
